src/Topology.v
@@ -9,27 +9,27 @@ Section Tree.
   Inductive Tree :=
   | Node: IdxT -> t -> list Tree -> Tree.
 
-  Fixpoint indicesOf (tr: Tree) :=
+  Fixpoint trIndicesOf (tr: Tree) :=
     match tr with
-    | Node i _ chd => i :: concat (map indicesOf chd)
+    | Node i _ chd => i :: concat (map trIndicesOf chd)
     end.
 
-  Definition curIdxOf (tr: Tree) :=
+  Definition trCurIdxOf (tr: Tree) :=
     match tr with
     | Node i _ _ => i
     end.
 
-  Definition valueOf (tr: Tree) :=
+  Definition trValueOf (tr: Tree) :=
     match tr with
     | Node _ v _ => v
     end.
 
-  Definition childrenOf (tr: Tree) :=
+  Definition trChildrenOf (tr: Tree) :=
     match tr with
     | Node _ _ chd => chd
     end.
 
-  Definition WfTree (tr: Tree) := NoDup (indicesOf tr).
+  Definition WfTree (tr: Tree) := NoDup (trIndicesOf tr).
 
   Fixpoint trIterate (f: Tree -> bool) (tr: Tree) :=
     if f tr
@@ -46,19 +46,19 @@ Section Tree.
 
   Fixpoint getThis (tr: Tree) (idx: IdxT): option Tree :=
     trIterate (fun tr =>
-                 if curIdxOf tr ==n idx
+                 if trCurIdxOf tr ==n idx
                  then true else false) tr.
 
   Fixpoint getParent (tr: Tree) (idx: IdxT): option Tree :=
     trIterate (fun tr =>
-                 if idx ?<n (map curIdxOf (childrenOf tr))
+                 if idx ?<n (map trCurIdxOf (trChildrenOf tr))
                  then true else false) tr.
 
   Definition getParentFwds (tr: Tree) (this: IdxT): list (IdxT * list IdxT) :=
     match getThis tr this with
     | Some ttr =>
       match getParent tr this with
-      | Some ptr => (curIdxOf ptr, removeL eq_nat_dec (indicesOf tr) (indicesOf ttr)) :: nil
+      | Some ptr => (trCurIdxOf ptr, removeL eq_nat_dec (trIndicesOf tr) (trIndicesOf ttr)) :: nil
       | None => nil
       end
     | None => nil
@@ -70,7 +70,7 @@ Section Tree.
       match ttr with
       | Node _ _ chd =>
         filter (fun ii => if fst ii ==n fch then false else true)
-               (map (fun tr => (curIdxOf tr, indicesOf tr)) chd)
+               (map (fun tr => (trCurIdxOf tr, trIndicesOf tr)) chd)
       end
     | None => nil
     end.
